<?xml version="1.0" encoding="UTF-8"?>

<section xml:id="sec-group-algebra" xmlns:xi="http://www.w3.org/2001/XInclude">
  <title>Group algebra</title>
  <definition xml:id="def-group-algebra">
    <title>Group Ring</title>
    
    
    <statement>
        <p>
            Let <m>R</m> be a commutative ring with unity and <m>G</m> a group. Consider the following set.
            <me>
                RG=\{\phi\in\Hom{Sets}{G}{R}:\phi(g)=0\quad\text{for all but finitely many }\,g\in G\}
            </me>
            Define <sq>addition</sq> and <sq>scalar multiplication</sq> in <m>RG</m> as follows.
            <me>
                (\phi r+\psi s)(g)=\phi(g)r+\psi(g)s
            </me>
            The <sq>multiplication</sq> in <m>RG</m> is defined as convolution product.
            <me>
                (\phi\psi)(g)=\sum \phi(h)\psi(h^{-1}g)\quad\text{such that}\quad h\in G,\text{ and } \phi(h)\psi(h^{-1}g)\neq 0
            </me>
            
        </p>
    </statement>
  </definition>
  <exercise>
    <statement>
        <p>
            Show that <m>RG</m> is closed under addition, scalar multiplication, and it is an <m>R</m>-module. Furthermore, show that multiplication is bilinear.
        </p>
    </statement>
  </exercise>
  <p>
    We now proceed to check the associativity of multiplication and the existence of unity in <m>RG</m>. We first observe that <m>RG</m> is a free <m>R</m>-module.
  </p>
  <proposition xml:id="prop-group-algebra-free-module">
    <statement>
        <p>
            Keep notations of <xref ref="def-group-algebra"/> above. Let for <m>g\in G</m>, <m>\chi_g</m> be the characteristic function of <m>g</m>, i.e., <m>\chi_g(h)=0</m> if <m>h\neq g</m> and <m>\chi_g(g)=1</m>. Then, set <m>\{\chi_g:g\in G\}</m> is an <m>R</m>-basis of <m>RG</m>. In particular, <m>RG</m> is a free <m>R</m>-module.
        </p>
        <p>
            Furthermore, <m>G\to RG</m> given by <m>g\mapsto\chi_g</m> is a monoid homomorphism. In particular, <m>\chi_g\chi_h=\chi_{gh}</m> and if <m>e\in G</m> is the identity then, <m>\chi_e</m> is the unity in <m>RG</m>.
        </p>
    </statement>
  </proposition>
  <proof>
    <p>
        Suppose that <m>\sum\chi_{g_i}r_i=0</m> for some <m>g_i\in G</m> and <m>r_i\in R</m>. Evaluating at <m>g_j</m>, we get <m>r_j=0</m>. Thus, the set is linearly independent. Now, let <m>\phi\in RG</m>. Then, we can write <m>\phi=\sum\chi_g\phi(g)</m> where the sum is over all <m>g\in G</m> such that <m>\phi(g)\neq 0</m>. This shows that the set spans <m>RG</m>. Thus, it is an <m>R</m>-basis of <m>RG</m>.
    </p>
    <p>
        Direct calculation shows that <m>\chi_g\chi_h=\chi_{gh}</m> for all <m>g,h\in G</m>.
    </p>
    <p>
        We show the associativity of multiplication. Let <m>\phi,\psi,\zeta\in RG</m>. Then, there exists <m>r_i,s_j,t_k\in R</m> such that <m>\phi=\sum\chi_{g_i}r_i</m>, <m>\psi=\sum\chi_{g_j}s_j</m>, <m>\zeta=\sum\chi_{g_k}t_k</m>. Therefore, we obtain the following.
        <md>
            <mrow> \left(\phi\psi\right)\zeta\amp =\left(\left(\sum\chi_{g_i}r_i\right)\left(\sum\chi_{g_j}s_j\right)\right)\sum\chi_{g_k}t_k</mrow>
            <mrow> \amp = \sum\left((\chi_{g_i}\chi_{g_j})\chi_{g_k}\right)(r_is_jt_k)</mrow>
            <mrow> \amp =\sum\chi_{g_i}\left(\chi_{g_j}\chi_{g_k}\right)(r_is_jt_k) </mrow>
            <mrow> \amp =\phi\left(\psi\zeta\right)</mrow>
        </md>
        This shows the associativity of multiplication.
    </p>
    <p>
        For any <m>\chi_{g_i}a_i\in RG</m> we get the following.
        <md>
            <mrow>\left((\chi_{g_i}a_i)\chi_e\right)(h) \amp =\sum\chi_{g_i}a_i(x)\chi_e(x^{-1}h)</mrow>
        </md>
        The above equation is nonzero only when <m>x=g_i</m> and <m>x^{-1}h=e</m>. This implies that <m>h=g_i</m>. Thus, we get <m>\left((\chi_{g_i}a_i)\chi_e\right)(h)=\chi_{g_i}a_i(h)</m>. Similarly, we can show that <m>\left(\chi_e(\chi_{g_i}a_i)\right)(h)=\chi_{g_i}a_i(h)</m>. This shows that <m>\chi_e</m> is the unity in <m>RG</m>.
    </p>
  </proof>
  <example xml:id="eg-group-algebra-cyclic-2">
    <title>Group algebra of the cyclic group of order 2</title>
    <statement>
        <p>
            Suppose that <m>C_2=\{\pm 1\}</m> denotes the cyclic group of order two. The general element of <m>\Z C_2</m> is of the form <m>a\chi_1 + b\chi_{-1}</m> for some <m>a,b\in\Z</m>. Observe that <m>\chi_{-1}^k=\chi_{(-1)^k}</m>, and that <m>\Z C_2</m> is commutative. Consider the map <m>\varphi=\Z[x]\to\Z C_2</m> given as follows.
            <me>
                a_0+a_1x+\cdots+a_nx^n\mapsto a_0\chi_1+a_1\chi_{-1}+a_2\chi_{(-1)^2}+\cdots+a_n\chi_{(-1)^n}
            </me>
            Check that the above map is a surjective homomorphism of rings. We compute its kernel.
            <me>
                \ker\varphi=\left\{\sum_{i=0}^n a_ix^i\in\Z[x]: a_0\chi_1+a_1\chi_{-1}+\cdots+a_n\chi_{(-1)^n}=0\right\}
            </me>
            We have <m>x^2-1\in\ker\varphi</m>. We claim that the kernel is generated by <m>x^2-1</m>. Let <m>f(x)=\sum_{i=0}^n a_ix^i\in\ker\varphi</m>. Then, <m>\left(\sum_{k\text{ even}}a_k\right)\chi_1+\left(\sum_{\ell\text{ odd}}a_\ell\right)\chi_{-1}=0</m>. As <m>\{\chi_1,\chi_{-1}\}</m> is a <m>\Z</m> basis we have that <m>\sum_{k\text{ even}}a_k=0</m> and <m>\sum_{\ell\text{ odd}}a_\ell=0</m>. Note that <m>f(1)=\sum_{k\text{ even}}a_k+\sum_{\ell\text{ odd}}a_\ell=0</m>, and that <m>\sum_{k\text{ even}}a_k-\sum_{\ell\text{ odd}}a_\ell=0</m>. Hence, <m>x-1</m> and <m>x+1</m> divides <m>f(x)</m>. As <m>x-1</m> and <m>x+1</m> are coprime, we get that <m>(x-1)(x+1)=x^2-1</m> divides <m>f(x)</m>. This shows that <m>\ker\varphi=(x^2-1)</m>. By the first isomorphism theorem, <m>\varphi</m> induces isomorphism of rings <m>\Z[x]/(x^2-1)\cong\Z C_2</m>.
        </p>
    </statement>
  </example>
  <exercise>
    <statement>
        <p>
            Let <m>G</m> be a group of order two. Show that <m>\Q G\simeq \Q\times \Q</m> via the map <me>\chi_1\cdot r+\chi_{-1}\cdot s\mapsto (r+s,r-s)</me>.
        </p>
    </statement>
  </exercise>
  <exercise>
    <statement>
        <p>
            Let <m>G</m> be a finite group. Show that in a group ring <m>\Z G</m> following holds.
            <ol>
                <li>
                    <p>
                        <m>f=\sum_{g\in G}\chi_g</m> satisfies <m>f^2=f</m>
                    </p>
                </li>
                <li>
                    <p>
                        <m>f\neq 0</m> and <m>1-f\neq 0</m>
                    </p>
                </li>
                <li>
                    <p>
                        <m>f(1-f)=0</m>
                    </p>
                </li>
            </ol>
        </p>
    </statement>
  </exercise>
  <theorem xml:id="thm-universal-property-group-algebra">
    <statement>
        <p>
            Suppose that <m>G</m> is a group and that <m>R</m> is a commutative ring. Then, <m>RG</m> is an <m>R</m>-algebra, and it is a free <m>R</m>-module with basis <m>\{\chi_g\mid g\in G\}</m>.
        </p>
        <p>
            Let <m>A</m> be an <m>R</m>-algebra, and let <m>\phi\colon G\to A</m> be a homomorphism to the multiplicative monoid of <m>A</m>. Then, <m>\phi</m> extends uniquely to an <m>R</m>-algebra homomorphism <m>\phi\colon RG\to A</m> of <m>R</m>-algebras.
        </p>
        <p>
            In other words, the following diagram commutes.
                <figure xml:id="fig-universal-property-group-algebra">
                    <caption>Universal property of group algebra</caption>
                    <image width="40%">
                        <latex-image>
                            \begin{tikzcd}
	                            G \amp\amp RG \\
	                                    \\
	                            A
	                            \arrow["{g\mapsto\chi_g}", from=1-1, to=1-3]
	                            \arrow["\phi"', from=1-1, to=3-1]
	                            \arrow[dashed, from=1-3, to=3-1]
                                \end{tikzcd}
                        </latex-image>
                    </image>
                    </figure>
                </p>
    </statement>
  </theorem>
  <proof>
    <p>
        In view of <xref ref="prop-group-algebra-free-module"/>, it suffices to show the universal property. Let <m>A</m> be an <m>R</m>-algebra and let <m>\phi\colon G\to A</m> be a homomorphism to the multiplicative monoid of <m>A</m>. Define <m>\tilde{\phi}\colon RG\to A</m> as follows.
        <me>
            \tilde{\phi}\left(\sum\chi_gr_g\right)=\sum\phi(g)r_g
        </me>
        We leave it to the reader to check that <m>\tilde{\phi}</m> is a well-defined homomorphism of <m>R</m>-algebras and that it is the unique extension of <m>\phi</m>.
    </p>
  </proof>
  <definition xml:id="def-augmentation-ideal">
    <title>Augmentation Ideal</title>
    <statement>
        <p>
            Let <m>R</m> be a commutative ring with unity and <m>G</m> a nontrivial group. The <em>augmentation map</em> is the <m>R</m>-algebra homomorphism <m>\epsilon:RG\to R</m> given by <m>\epsilon(\sum\chi_gr_g)=\sum r_g</m>. The kernel of the augmentation map is called the <em>augmentation ideal</em> of <m>RG</m>, and it is denoted by <m>I(G)</m>.
        </p>
    </statement>
  </definition>
  <exercise>
    <title>Augmentation map is an <m>R</m>-algebra homomorphism</title>
    <statement>
        <p>
            Show that the augmentation map <m>\epsilon:RG\to R</m> is a well-defined surjective <m>R</m>-algebra homomorphism.
        </p>
    </statement>
  </exercise>
  <exercise xml:id="exe-augmentation-ideal-generators">
    <title>Generators of augmentation ideal</title>
    <statement>
        <p>
            Let <m>R</m> be a commutative ring with unity and <m>G</m> a nontrivial group. Show that the augmentation ideal <m>I(G)</m> is generated as an <m>R</m>-module by the set <m>\{\chi_g-\chi_e:g\in G,g\neq e\}</m>, where <m>e</m> is the identity of <m>G</m>.
        </p>
    </statement>
  </exercise>
</section>